src/QueryStructure/Specification/Operations/Update.v
@@ -110,17 +110,27 @@ Definition QSUpdate (qs : QueryStructureHint) Ridx
            (UpdateFunction : (@Tuple (schemaHeading (QSGetNRelSchema _ Ridx))) ->
                              (@Tuple (schemaHeading (QSGetNRelSchema _ Ridx)))) :=
   (qs'       <- Pick (QSUpdateSpec _ Ridx UpdatedTuples UpdateFunction);
-   b         <- Pick (SuccessfulUpdateSpec _ Ridx qs' UpdatedTuples UpdateFunction);
-   ret (qs', b))%comp.
+   deleted   <- Pick (UnIndexedEnsembleListEquivalence
+                        (Intersection _
+                                      (GetRelation qsHint Ridx)
+                                      (fun x => UpdatedTuples (indexedElement x))));
+   ret (qs', deleted))%comp.
 
 Opaque QSUpdate.
 
-Variable UpdateTuple : forall (attrs: list Attribute) (attr: Attribute) (value: Component attr),
+Variable UpdateTuple : forall (attrs: list Attribute) (attr: Attribute),
+                         (Component attr -> Component attr) ->
                          @Tuple (BuildHeading attrs) -> @Tuple (BuildHeading attrs).
 
-Notation "a := b" := (UpdateTuple _ {|bindex := a|} (a::b)) (at level 80).
-Notation "[ a ; .. ; c ]" := (compose a .. (compose c id) ..).
+Notation "a |= b" := (@UpdateTuple _ {|attrName := a; attrType := _|}
+                             (fun _ => Build_Component (_::_) b%list)) (at level 80).
+Notation "a ++= b" := (@UpdateTuple _ {|attrName := a; attrType := string|}
+                             (fun o => Build_Component (_::_) (append (value o) b))) (at level 80).
+Notation "a :+= b" := (@UpdateTuple _ {|attrName := a; attrType := list _|}
+                             (fun o => Build_Component (_::_) (cons b (value o)))) (at level 80).
+Notation "[ a ; .. ; c ]" := (compose a .. (compose c id) ..) : Update_scope.
 
-Notation "'Update' b 'from' Ridx 'set' Trans 'where' Ens" :=
-  (QSUpdate _ {|bindex := Ridx%comp |} (fun b => Ens) Trans)
+Delimit Scope Update_scope with Update.
+Notation "'UpdateX' b 'from' Ridx 'making' Trans 'where' Ens" :=
+  (QSUpdate _ {|bindex := Ridx%comp |} (fun b => Ens) Trans%Update)
     (at level 80) : QuerySpec_scope.
