src/QueryStructure/Specification/Representation/QueryStructureNotations.v
@@ -1,7 +1,7 @@
 Require Export Coq.Strings.String Coq.omega.Omega Coq.Lists.List Coq.Logic.FunctionalExtensionality Coq.Sets.Ensembles
         ADTSynthesis.Common.Ensembles.IndexedEnsembles
         ADTSynthesis.Computation ADTSynthesis.ADT ADTSynthesis.ADTRefinement ADTSynthesis.ADTNotation ADTSynthesis.QueryStructure.Specification.Representation.QueryStructureSchema
-        ADTSynthesis.ADTRefinement.BuildADTRefinements ADTSynthesis.QueryStructure.Specification.Operations.Query ADTSynthesis.QueryStructure.Specification.Operations.Insert ADTSynthesis.QueryStructure.Specification.Operations.Empty (* Add Update *)
+        ADTSynthesis.ADTRefinement.BuildADTRefinements ADTSynthesis.QueryStructure.Specification.Operations.Query ADTSynthesis.QueryStructure.Specification.Operations.Insert ADTSynthesis.QueryStructure.Specification.Operations.Empty ADTSynthesis.QueryStructure.Specification.Operations.Update
         ADTSynthesis.QueryStructure.Specification.Operations.Delete ADTSynthesis.QueryStructure.Specification.Representation.QueryStructure.
 
 Notation "heading / attr_index" := ((fun x : Attributes heading => x)
